some fixes for ParseInt and ReMatch

parser/parseInt.dfy
@@ -1,4 +1,5 @@
 module ParseInt {
+    import Dafny.Collections.Seq
     function power(x: int, i: nat): int {
         if i == 0 then 1 else if i == 1 then x else x * power(x, i-1)
     }
@@ -6,11 +7,12 @@ module ParseInt {
     function integerHelper(ns: string, sum: int, negative: bool): int {
         if |ns| == 0 then if negative then 0 - sum else sum
         else if ns[0] == '-' then integerHelper(ns[1..], sum, true)
-        else integerHelper(ns[1..], sum + ((ns[0] as int) - 48) * power(10, |ns|-1), negative)
+        else if 48 <= (ns[0] as int) < 58 then integerHelper(ns[1..], sum + ((ns[0] as int) - 48) * power(10, |ns|-1), negative)
+        else integerHelper(ns[1..], sum, negative)
     }
 
     function Integer(ns: string): int {
-        integerHelper(ns, 0, false)
+        integerHelper(Seq.Filter(x => 48 <= (x as int) < 58,ns), 0, false)
     }
 
     method toInt(ns: string) returns (ret: int) 
@@ -48,16 +50,16 @@ module ParseInt {
         {
             var digit := i % 10; 
             // assert lookup[digit] in numchars();
-            ret := ret+[lookup[digit]];
+            ret := [lookup[digit]]+ret;
             i := i / 10;
         }
         return ret;
     }
 
     function numchars(): seq<char>
-        ensures numchars() == ['-','0','1','2','3','4','5','6','7','8','9']
+        ensures numchars() == ['0','1','2','3','4','5','6','7','8','9','-']
     {
-        ['-','0','1','2','3','4','5','6','7','8','9']
+        ['0','1','2','3','4','5','6','7','8','9','-']
     }
 
     predicate charInNC(c: char) {
@@ -68,4 +70,8 @@ module ParseInt {
     {
         s == "" || forall i  :: 0 <= i < |s| ==> charInNC(s[i])
     }
+
+    export
+        provides Integer
+        provides toInt, toStr, isNumString
 }
